@base <https://raw.githubusercontent.com/beatestermann/glam-inventory/master/> .
@prefix owl: <http://www.w3.org/2002/07/owl#> .
@prefix rdf: <http://www.w3.org/1999/02/22-rdf-syntax-ns#> .
@prefix xml: <http://www.w3.org/XML/1998/namespace> .
@prefix xsd: <http://www.w3.org/2001/XMLSchema#> .
@prefix rdfs: <http://www.w3.org/2000/01/rdf-schema#> .
@prefix schema: <http://schema.org/> .
@prefix skos: <http://www.w3.org/2004/02/skos/core#> .
@prefix dct: <http://purl.org/dc/terms/> .
@prefix org: <http://www.w3.org/ns/org#> .
@prefix foaf: <http://xmlns.com/foaf/0.1/> .
@prefix dbp: <http://dbpedia.org/property/> .
@prefix dc: <http://purl.org/dc/elements/1.1/> .

    
    
<glam-vocabulary.ttl> a owl:Ontology; 
    dc:title "GLAM Inventory Vocabulary (OpenGLAM CH)"@en;
    dc:description "This vocuabulary extends the Foaf, Schema, Dublin Core Terms, and other existing vocabularies by specifying further classes and properties related to the heritage domain that are relevant for the description of the Swiss GLAM Inventory (inventory of heritage institutions) and are not specified elsewhere."@en;
    owl:versionInfo "0.1 (Draft)";
    dct:issued "";
    dct:modified "";
    dc:creator "Beat Estermann";
    dc:creator "Oskari Romanoff";
    dc:publisher "Open GLAM CH Working Group";
    dct:rights "Copyright by the authors, available under the Creative Commons Attribution License http://creativecommons.org/licenses/by/4.0". 
    

#################################################################
#
#    Classes
#
#################################################################

     
<HeritageCollection> a owl:Class;
    dct:description "Collection of heritage objects held by a heritage institution whose mission it is to preserve the collection for future generations.";
    skos:prefLabel "heritage collection"@en;
    skos:definition "Collection of heritage objects held by a heritage institution whose mission it is to preserve the collection for future generations."@en.
    
    
#################################################################
#
#    Object Properties
#
#################################################################

    

   



#################################################################
#
#    Datatype Properties
#
#################################################################




# Datatype Properties related to schema:Organization

<hasGLAMIdentifier> a owl:DatatypeProperty;
    dct:description "Unique identifier for galleries, libraries, archives, museums, and other heritage institutions as used in the context of the OpenGLAM Benchmark Survey.";
    skos:prefLabel "GLAM identifier"@en;
    rdfs:domain schema:Organization;
    rdfs:subPropertyOf dct:identifier;
    skos:definition "Unique identifier for galleries, libraries, archives, museums, and other heritage institutions as used in the context of the OpenGLAM Benchmark Survey."@en.


<primaryInstitutionType> a owl:ObjectProperty;
    dct:description "Primary type of heritage institution (aka: 'museum', 'library', 'archive / records office', 'other'";
    skos:prefLabel "primary institution type"@en;
    rdfs:domain schema:Organization; 
    skos:definition "Primary type of heritage institution (aka: 'museum', 'library', 'archive / records office', 'other'"@en.

    
<secondaryInstitutionType> a owl:ObjectProperty;
    dct:description "More detailed type of heritage institution (e.g. 'museum of art', 'museum of science and technology', etc.)";
    skos:prefLabel "institution type"@en;
    rdfs:domain schema:Organization;
    skos:definition "More detailed type of heritage institution (e.g. 'museum of art', 'museum of science and technology', etc.)"@en.




# Datatype Properties related to <HeritageCollection>

<hasPCPNumber> a owl:DatatypeProperty;
    dct:description "PCP reference number. Identifier for cultural properties in Switzerland.";
    skos:prefLabel "PCP reference number"@en;
    rdfs:domain <HeritageCollection>;
    rdfs:subPropertyOf dct:identifier;
    skos:definition "PCP reference number. Identifier for cultural properties in Switzerland."@en.

        
<hasPCPCategory> a owl:ObjectProperty;
    dct:description "Category for cultural properties in Switzerland ('A' = 'cultural property of national significance'; 'B' = 'cultural property of regional significance'";
    skos:prefLabel "PCP category"@en;
    rdfs:domain <HeritageCollection>;
    rdfs:subPropertyOf <PCP-NO>;
    skos:definition "Category for cultural properties in Switzerland ('A' = 'cultural property of national significance'; 'B' = 'cultural property of regional significance'"@en.
